# Currying
## Motivation
Look again at the summation functions:

```scala
def sumInts(a: Int, b: Int)       = sum(x => x, a, b)
def subCubes(a: Int, b: Int)      = sum(x => x * x * x, a, b)
def sumFactorials(a: Int, b: Int) = sum(fact, a, b)
```
**Question:** Note that `a` and `b` get passed unchanged from `sumInts` and `sumCubes` into `sum`. Can we be even shorter by getting rid of these parameters?

## Functions Returning Functinos
Let's rewrite `sum` as follows:

```scala
def sum(f: Int => Int): (Int, Int) => Int = {
	def sumF(a: Int, b: Int): Int = 
		if (a > b) 0
		else f(a) + sumF(a + 1, b)
	sumF
}
```
`sum` is now a function that returns another function. The returned function `sumF` applies the given function parameter `f` and sums the results.

## Stepwise Applications
We can then define:

```scala
def sumInts       = sum(x => x)
def sumCubes      = sum(x => x * x * x)
def sumFactorials = sum(fact)
```
These functions can in turn be applied like any other function:

```scala
sumCubes(1, 10) + sumFactorial(10, 20)
```

## Consecutive Stepwise Applications
In the previous example, can we avoid the `sumInts`, `sumCubes`, ... middlemen?  
Of coures:

```scala
sum(cube)(1, 10)
```

* `sum(cube)` applies `sum` to `cube` and returns the *sum of cubes* function.
* `sum(cube)` is therefore equivalent to `sumCubes`.
* This function is next applied to the arguments `(1, 10)`.

Generally, function application associates to the left:

```scala
sum(cube)(1, 10) == (sum(cube))(1, 10)
```

## Multiple Parameter Lists
The definition of functions that return functions is so useful in functional programming that there is a special syntax for it in Scala. For example, the following definition of `sum` is equivalent to the one with the nested `sumF` function, but shorter:

```scala
def sum(f: Int => Int)(a: Int, b: Int): Int = 
	if (a > b) 0 else f(a) + sum(f)(a + 1, b) 
```

## Expansion of Multiple Parameter Lists
In general, a definition of a function with multiple parameter lists

```scala
def f(args_1)...(args_n) = E
```
where `n > 1`, is equivalent to 

```scala
def f(args_1)...(args_n-1) = { def g(args_n) = E; g }
```
where `g` is a fresh identifier. Or for short:

```scala
def f(args_1)...(args_n-1) = (args_n => E)
```
By repeating the process *n* times

```scala
def f(args_1)...(args_n-1)(args_n) = E
```
is shown to be equivalent to 

```scala
def f = (args_1 => (args_2 => ... (args_n => E)...))
```
This style of definition and function application is called *currying*, named for its instigator, Haskell Brooks Curry (1900-1982), a twentieth century logician. In fact, the idea goes back even further to SchoÌˆnfinkel and Frege, but the term "currying" has stuck.

## More Function Types
Question: Given,

```scala 
def sum(f: Int => Int)(a: Int, b: Int): Int = ...
```
What is the type of `sum`?  
**Answer:**

```scala
(Int=>Int) => (Int, Int) => Int
```
Note that functinoal types associate to the right, That is to say that

```scala
Int => Int => Int
```
is equivalent to 

```scala
Int => (Int => Int)
```

## Exercise
1. Write a `product` function that calcuates the product of the values of a function for the points on a given interval.
2. Write `factorial` in terms of `product`.
3. Can you write a more genral function, which generalizes both `sum` and `product`?

```scala
def product(f: Int => Int)(a: Int, b: Int): Int = 
	if (a > b) 1 
	else f(a) * product(f)(a + 1, b)
	
def factorial(n: Int) = product(x => x)(1, n)

def mapReduce(f: Int => Int, combine: (Int, Int) => Int, zero: Int)(a: Int, b: Int): Int =
	if (a > b) zero
	else combine(f(a), mapReduce(f, combine, zero)(a + 1, b))
```